# Lecture 12 - Notes  

**January 29, 2016**  

## Eigenfunctions - Continued

_definition_: Given a system $y[n] = H\left(e^{j \omega}\right) e^{j \omega n}$ with an impulse response $h[n]$, the __frequency response__ is,

$$\begin{align}
    H\left(e^{j \omega}\right) = \sum_{n = -\infty}^{\infty} h[n] e^{-j \omega n}
\end{align}$$

Given a difference equation,

$$\begin{align}
    \sum_{i=0}^{M} b_i x[n - i] = \sum_{j=0}^{N} a_j y[n-j]
\end{align}$$

the frequency response is,


$$\begin{align}
    H\left(e^{j \omega}\right) = \frac{\sum_{i=0}^{M} b_i e^{-j \omega i}}{\sum_{k=0}^{N} a_k e^{-j \omega k}}
\end{align}$$

#### Examples

*Is $3^n$ an eigenfunction?*

Yes. Since $3^n = \left(3e^{j0}\right)^n$.

*Is $\cos{\omega_0 n}$ an eigenfunction?*

No.

### Sinusoidal System Responses

Suppose, $x[n] = A \cos{\omega_0 n + \varphi}$, then


$$\begin{align}
    x[n] &= A \cos{\omega_0 n + \varphi} \\\\
    &= \frac{A}{2}\left( e^{j(\omega_0 n + \varphi)} + e^{-j(\omega_0 n + \varphi)} \right) \\\\
    &= \frac{A}{2}\left( e^{j\omega_0 n}e^{j\varphi} + e^{-j\omega_0 n}e^{j\varphi} \right) \\\\
    &= \frac{A}{2} e^{j\omega_0 n}e^{j\varphi} + \frac{A}{2} e^{j\omega_0 n}e^{-j\varphi} \\\\
    &\xrightarrow{S} \frac{A}{2} e^{j\varphi} H\left(e^{j \omega_0}\right) e^{j\omega_0 n} + \frac{A}{2} e^{-j\varphi} H\left(e^{-j \omega_0}\right) e^{j\omega_0 n}  \\\\
\end{align}$$

This gives us,

$$\begin{align}
    y[n] &= \frac{A}{2} e^{j\varphi} H\left(e^{j \omega_0}\right) e^{j\omega_0 n} + \frac{A}{2} e^{-j\varphi} H\left(e^{-j \omega_0}\right) e^{j\omega_0 n} \\\\
    &= A \left|H\left( e^{j \omega_0} \right)\right|\cos{\left(\omega_0 n + \varphi - \theta_0\right)}
\end{align}$$


