# Lecture 13 - Notes  

**February 3, 2016**  

## The Discrete-Time Fourier Transform

_definition_: We define the __Discrete-Time Fourier Transform__ as,

$$
    X\left( e^{j\omega} \right) = \sum_{k = -\infty}^{\infty} x[k]e^{-j \omega k}
$$

and the inverse transform,

$$\begin{align}
    x[n] = \frac{1}{2\pi} \int_{-\pi}^{\pi} X\left(e^{j\omega}\right) e^{j \omega n} ~d\omega
\end{align}$$

#### Example

Find the Fourier transform of,

$$\begin{align}
    x[n] = a^n u[n]
\end{align}$$

where $|a| \lt 1$.

So,


$$\begin{align}
    X\left( e^{j\omega} \right) &= \sum_{k = -\infty}^{\infty} x[k]e^{-j \omega k} \\\\ 
    &= \sum_{k = -\infty}^{\infty} a^k u[k] e^{-j \omega k} \\\\
    &= \sum_{k = 0}^{\infty} a^k e^{-j \omega k} \\\\
    &= \sum_{k = 0}^{\infty} \left( a e^{-j \omega} \right)^k \\\\
    &= \frac{1}{1 - a e^{-j \omega}} \\\\
\end{align}$$

#### Example

Find the inverse Fourier transform of,

$$\begin{align}
    X\left(e^{j\omega}\right) = 1 + 3e^{-j\omega} + 2e^{-j2\omega} - 4e^{-j3\omega} + e^{-j10\omega}
\end{align}$$

Using the properties of Fourier transforms,

$$\begin{align}
    x[n] = \underbrace{\delta[n]}_{1} + 
           \underbrace{3\delta[n-1]}_{3e^{-j \omega}} + 
           \underbrace{2\delta[n-2]}_{2e^{-j2\omega}} - 
           \underbrace{4\delta[n-3]}_{4e^{-j3\omega}} + 
           \underbrace{\delta[n-10]}_{e^{-j10\omega}}
\end{align}$$

