# Lecture 15 - Notes  

**February 17, 2016**  

## Properties of Fourier Transforms

### Symmetry

For an arbitrary $x[n]$,

$$\begin{align}
    x[n] = \underbrace{x_\text{even}[n]}_{X_R\left(e^{j\omega}\right)} + \underbrace{x_\text{odd}[n]}_{X_I\left(e^{j\omega}\right)}
\end{align}$$
 
 If,

$$\begin{gather}
    \left| X\left(e^{j\omega}\right) \right| = \left| X\left(e^{-j\omega}\right) \right| \\
\end{gather}$$

then $x[n]$ is even. If,


$$\begin{align}
    \angle X\left(e^{j\omega}\right) = \angle X\left(e^{-j\omega}\right)
\end{align}$$

then $x[n]$ is odd.

### Time and Frequency Shifting

To shift in the time domain,


$$\begin{align}
    x[n - n_d] \overset F \longleftrightarrow e^{-jwn_d} X \left( e^{j\omega} \right)
\end{align}$$

To shift in the frequency domain,



### Frequency Differentiation

To differentiate in the frequency domain,

$$\begin{align}
    nx[n] \overset F \longleftrightarrow j \frac{d X \left( e^{j\omega} \right)}{d\omega}
\end{align}$$

##### Example

Find $X \left( e^{j\omega} \right)$ of,

$$\begin{align}
    x[n] = (n - 1)\left( \frac{1}{3} \right)^{\left| n \right|}
\end{align}$$

###### Solution

Let,

$$\begin{align}
    x_1[n] &= \left( \frac{1}{3} \right)^{\left| n \right|} \\\\
    &= \begin{cases} 
      \left( \frac{1}{3} \right)^{ n} & n \ge 0 \\\\
      \left( \frac{1}{3} \right)^{-n} & n \lt 0 \\\\
   \end{cases}
\end{align}$$ 

so,

$$\begin{align}
    X_1 \left( e^{j\omega} \right) &= \sum_{n = -\infty}^{\infty} \left( \frac{1}{3} \right)^{|n|} e^{-j\omega n} \\\\
    &= \sum_{n = -\infty}^{0} \left( \frac{1}{3} \right)^{-n} e^{-j\omega n} + \sum_{n = 0}^{\infty} \left( \frac{1}{3} \right)^{n} e^{-j\omega n} - 1 \\\\
    &= \sum_{p = 0}^{\infty} \left( \frac{1}{3} \right)^{p} e^{j\omega p} + \sum_{n = 0}^{\infty} \left( \frac{1}{3} \right)^{n} e^{-j\omega n} - 1 \\\\
    &= \frac{1}{1 - \frac{1}{3} e^{j\omega}} + \frac{1}{1 - \frac{1}{3} e^{-j\omega}} - 1 \\\\
    &= \frac{4}{5 - 3 \cos{\omega}}
\end{align}$$

now,

$$\begin{align}
    x[n] &= n x_1[n] - x_1[n] \\\\
    X \left( e^{j\omega} \right) &= j \frac{d X_1 \left( e^{j\omega} \right)}{d\omega} - X_1 \left( e^{j\omega} \right) \\\\
    &~~\vdots \\\\
    &= \frac{4}{5 - 3 \cos{\omega}} - j \frac{12 \sin{\omega}}{\left(5 - 3 \cos{\omega} \right)^2}
\end{align}$$

### Convolution

To transform convolution in the time domain into the frequency domain,

$$\begin{align}
    x_1[n] &\overset F \longleftrightarrow X_1 \left( e^{j\omega} \right) \\\\
    x_2[n] &\overset F \longleftrightarrow X_2 \left( e^{j\omega} \right) \\\\
    &~~\downarrow \\\\
    x_1[n] * x_2[n] &\overset F \longleftrightarrow X_1 \left( e^{j\omega} \right)X_2 \left( e^{j\omega} \right) \\\\
\end{align}$$

