# Lecture 20 - Notes  

**March 1, 2016**  

## The Inverse Z-Transform

If we express the Z-transform as a Fourier Transform of an equally weighted sequence,

$$\begin{aligned}
    x[n] = \frac{1}{2 \pi j} \oint X(z) z^{n-1} ~dz
\end{aligned}$$ 

For rational Z-transforms we can compute the inverse Z-transforms alternate ways,

* [Inspection](#inspection)
* [Partial Fraction Expansion](#partial-fraction-expansion)
* [Power Series Expansion](#power-series-expansion)

### Inspection

Use a table of Z-transform properties and pairs to convert back to the time domain.

**e.g.**

*Determine $h[n]$ given,*

$$\begin{aligned}
    H(z) = \frac{1 - z^{-1}}{1 + \frac{3}{4} z^{-1}}
\end{aligned}$$

Consider,

$$\begin{aligned}
    H(z) &= \frac{1 - z^{-1}}{1 + \frac{3}{4} z^{-1}} \\\\
    &= \underbrace{\frac{1}{1 + \frac{3}{4} z^{-1}}}_\text{exponential} - \underbrace{\frac{z^{-1}}{1 + \frac{3}{4} z^{-1}}}_\text{shifted exponential} \\\\
    &\downarrow\\\\
    h[n] &= \left( \frac{3}{4} \right)^n u[n] - \left( \frac{3}{4} \right)^{n-1} u[n-1]
\end{aligned}$$

### Partial Fraction Expansion

Expand two sums which are partial fractions,

$$\begin{aligned}
    X(z) &= \frac{\sum_{k=0}^M b_k z^{-k}}{\sum_{k=0}^N a_k z^{-k}} \\\\
    &\downarrow \\\\
    X(z) &= \sum_{k=1}^N \frac{A_k}{1-d_k z^-1}
\end{aligned}$$

**e.g.**

*Determine the inverse Z-transform of,*

$$\begin{aligned}
    X(z) &= \frac{3z^2 - \frac{5}{6}z}{\left(z - \frac{1}{4}\right)\left(z - \frac{1}{3}\right)}
\end{aligned}$$

*where $\left| z \right| \lt \frac{1}{3}$.*

We identify $M = 1$ and $N = 2$ and perform the partial fraction expansion,

$$\begin{aligned}
    \frac{3z - \frac{5}{6}z}{\left(z - \frac{1}{4}\right)\left(z - \frac{1}{3}\right)} &= \frac{A}{\left(z - \frac{1}{4}\right)} + \frac{B}{\left(z - \frac{1}{3}\right)} \\\\
    3z^2 - \frac{5}{6}z  &= A \left(z - \frac{1}{3}\right) + B \left(z - \frac{1}{4}\right) \\\\
\end{aligned}$$

**TODO**


### Power Series Expansion

$$\begin{aligned}
    X(z) &= \frac{\sum_{k=0}^M b_k z^{-k}}{\sum_{k=0}^N a_k z^{-k}} \\\\
    &\downarrow \\\\
    X(z) &= \sum_{n=-\infty}^{+\infty} x[n]z^{-1}
\end{aligned}$$

**e.g.**

*Determine the inverse Z-transform of,*

$$\begin{aligned}
    X(z) &= (1 + 2z)(1 + 3z^{-1})
\end{aligned}$$

Start by expanding,

$$\begin{aligned}
    X(z) &= (1 + 2z)(1 + 3z^{-1}) \\\\
    &= 1 - 2z + 3z^{-1} + 6 \\\\
    &= 3z^{-1} + 7 - 2z \\\
    &\downarrow \\\\
    x[n] &= \begin{cases} 
      3 & n =  1 \\\\
      7 & n =  0 \\\\
      2 & n = -1 \\\\
   \end{cases}
\end{aligned}$$

**e.g.**

*Determine the inverse Z-transform of,*

$$\begin{aligned}
    X(z) &= \frac{1}{1 + \frac{1}{2}z^{-1}}
\end{aligned}$$

**TODO**
